deps/poulet4/lib/P4cub/Semantics/Dynamic/BigStep/Value/Equality.v
@@ -1,7 +1,6 @@
 Require Import Poulet4.P4cub.Semantics.Dynamic.BigStep.Value.Syntax
         Poulet4.P4cub.Semantics.Dynamic.BigStep.Value.IndPrincip
-        Coq.ZArith.BinInt Coq.NArith.BinNat
-        (*Poulet4.P4cub.Syntax.Syntax*).
+        Poulet4.P4cub.Syntax.Equality Coq.ZArith.BinInt Coq.NArith.BinNat.
 Import Val ValueNotations.
 
 (** Computational Value equality *)
@@ -18,20 +17,23 @@ Fixpoint eqbv (v1 v2 : v) : bool :=
   | Bit w1 n1, Bit w2 n2 => (w1 =? w2)%N && (n1 =? n2)%Z
   | Error err1, Error err2
     => if equiv_dec err1 err2 then true else false
-  | Struct vs1 b1, Struct vs2 b2
-    => if equiv_dec b1 b2 then lstruct vs1 vs2 else false
+  | Lists ls1 vs1, Lists ls2 vs2
+    => lists_eqb ls1 ls2 && lstruct vs1 vs2
   | _,          _          => false
   end.
-  
+
+Local Hint Rewrite eqb_reflx.
+Local Hint Rewrite equiv_dec_refl.
+Local Hint Rewrite Pos.eqb_refl.
+Local Hint Rewrite Z.eqb_refl.
+Local Hint Rewrite N.eqb_refl.
+Local Hint Rewrite andb_true_r.
+Local Hint Rewrite lists_eqb_refl.
+Local Hint Resolve lists_eqb_eq : core.
+Local Hint Extern 0 => equiv_dec_refl_tactic : core.
+
 Lemma eqbv_refl : forall V : v, eqbv V V = true.
 Proof.
-  Local Hint Rewrite eqb_reflx.
-  Local Hint Rewrite equiv_dec_refl.
-  Local Hint Rewrite Pos.eqb_refl.
-  Local Hint Rewrite Z.eqb_refl.
-  Local Hint Rewrite N.eqb_refl.
-  Local Hint Rewrite andb_true_r.
-  Local Hint Extern 0 => equiv_dec_refl_tactic : core.
   induction V using custom_v_ind; simpl in *;
     autorewrite with core; simpl; auto;
     try ind_list_Forall;
@@ -83,17 +85,19 @@ Proof.
             repeat eauto_too_dumb; subst; auto
         end.
 Qed.
-  
+
+Local Hint Resolve eqbv_refl : core.
+Local Hint Resolve eqbv_eq : core.
+
 Lemma eqbv_eq_iff : forall v1 v2 : v, eqbv v1 v2 = true <-> v1 = v2.
 Proof.
-  Local Hint Resolve eqbv_refl : core.
-  Local Hint Resolve eqbv_eq : core.
   intros; split; intros; subst; auto.
 Qed.
-  
+
+Local Hint Resolve eqbv_eq_iff : core.
+
 Lemma eqbv_reflect : forall v1 v2, reflect (v1 = v2) (eqbv v1 v2).
 Proof.
-  Local Hint Resolve eqbv_eq_iff : core.
   intros; reflect_split; auto; subst.
   rewrite eqbv_refl in Heqb; discriminate.
 Qed.
