deps/poulet4/lib/P4cub/Syntax/Substitution.v
@@ -12,121 +12,123 @@ Fixpoint tshift_t (n : nat) (τ : Expr.t) : Expr.t :=
   | Expr.TInt _
   | Expr.TError       => τ
   | Expr.TVar X       => n + X
-  | Expr.TStruct ts b => Expr.TStruct (map (tshift_t n) ts) b
+  | Expr.TArray s t   => Expr.TArray s (tshift_t n t)
+  | Expr.TStruct b ts => Expr.TStruct b (map (tshift_t n) ts)
   end.
 
-Definition exts (σ : nat -> Expr.t) (X : nat) : Expr.t :=
-  match X with
-  | O => O
-  | S n => tshift_t 1 $ σ n
-  end.
+Section Sub.
+  Variable σ : nat -> Expr.t.
 
-Fixpoint tsub_t (σ : nat -> Expr.t) (t : Expr.t) : Expr.t :=
-  match t with
-  | Expr.TBool
-  | Expr.TBit _
-  | Expr.TInt _
-  | Expr.TError       => t    
-  | Expr.TStruct ts b => Expr.TStruct (List.map (tsub_t σ) ts) b
-  | Expr.TVar X       => σ X
-  end.
+  Definition exts (X : nat) : Expr.t :=
+    match X with
+    | O => O
+    | S n => tshift_t 1 $ σ n
+    end.
 
-Fixpoint tsub_e (σ : nat -> Expr.t) (e : Expr.e) : Expr.e :=
-  match e with
-  | Expr.Bool _
-  | Expr.Bit _ _
-  | Expr.Int _ _
-  | Expr.Error _ => e
-  | Expr.Var t x       => Expr.Var (tsub_t σ t) x
-  | Expr.Slice e hi lo => Expr.Slice (tsub_e σ e) hi lo
-  | Expr.Cast t e      => Expr.Cast (tsub_t σ t) (tsub_e σ e)
-  | Expr.Uop rt op e => Expr.Uop (tsub_t σ rt) op (tsub_e σ e)
-  | Expr.Bop rt op e1 e2 =>
-      Expr.Bop (tsub_t σ rt) op (tsub_e σ e1) (tsub_e σ e2)
-  | Expr.Struct es ob =>
-      Expr.Struct (map (tsub_e σ) es) ob
-  | Expr.Member rt mem arg =>
-      Expr.Member (tsub_t σ rt) mem (tsub_e σ arg)
-  end.
+  Fixpoint tsub_t (t : Expr.t) : Expr.t :=
+    match t with
+    | Expr.TBool
+    | Expr.TBit _
+    | Expr.TInt _
+    | Expr.TError       => t
+    | Expr.TArray n t   => Expr.TArray n $ tsub_t t
+    | Expr.TStruct b ts => Expr.TStruct b $ List.map tsub_t ts
+    | Expr.TVar X       => σ X
+    end.
 
-Definition tsub_param (σ : nat -> Expr.t) (pa : paramarg Expr.t Expr.t) :=
-  match pa with
-  | PAIn t => PAIn (tsub_t σ t)
-  | PAOut t => PAOut (tsub_t σ t)
-  | PAInOut t => PAInOut (tsub_t σ t)
-  end.
+  Definition tsub_lists (l : Expr.lists) : Expr.lists :=
+    match l with
+    | Expr.lists_struct   => Expr.lists_struct
+    | Expr.lists_array  t => Expr.lists_array $ tsub_t t
+    | Expr.lists_header b => Expr.lists_header b
+    end.
 
-Definition tsub_arg (σ : nat -> Expr.t)
-  : paramarg Expr.e Expr.e -> paramarg Expr.e Expr.e :=
-  paramarg_map_same $ tsub_e σ.
+  Fixpoint tsub_e (e : Expr.e) : Expr.e :=
+    match e with
+    | Expr.Bool _
+    | Expr.Bit _ _
+    | Expr.Int _ _
+    | Expr.Error _ => e
+    | Expr.Var t x       => Expr.Var (tsub_t t) x
+    | Expr.Slice hi lo e => Expr.Slice hi lo $ tsub_e e
+    | Expr.Cast t e      => Expr.Cast (tsub_t t) $ tsub_e e
+    | Expr.Uop rt op e   => Expr.Uop (tsub_t rt) op $ tsub_e e
+    | Expr.Bop rt op e1 e2 =>
+        Expr.Bop (tsub_t rt) op (tsub_e e1) $ tsub_e e2
+    | Expr.Index t e1 e2 => Expr.Index (tsub_t t) (tsub_e e1) $ tsub_e e2
+    | Expr.Member rt mem arg =>
+        Expr.Member (tsub_t rt) mem (tsub_e arg)
+    | Expr.Lists l es => Expr.Lists (tsub_lists l) $ map tsub_e es
+    end.
+  
+  Definition tsub_param (pa : paramarg Expr.t Expr.t) :=
+    match pa with
+    | PAIn t => PAIn $ tsub_t t
+    | PAOut t => PAOut $ tsub_t t
+    | PAInOut t => PAInOut $ tsub_t t
+    end.
 
-Definition tsub_transition (σ : nat -> Expr.t) (transition : Parser.e) :=
-  match transition with
-  | Parser.Goto s =>
-      Parser.Goto s
-  | Parser.Select discriminee default cases =>
-      Parser.Select (tsub_e σ discriminee) default cases
-  end.
+  Definition tsub_arg
+    : paramarg Expr.e Expr.e -> paramarg Expr.e Expr.e :=
+    paramarg_map_same $ tsub_e.
 
-Definition tsub_fun_kind (σ : nat -> Expr.t) (fk : Stmt.fun_kind) : Stmt.fun_kind :=
-  match fk with
-  | Stmt.Funct f τs oe
-    => Stmt.Funct f (map (tsub_t σ) τs) $ option_map (tsub_e σ) oe
-  | Stmt.Action a cargs
-    => Stmt.Action a $ map (tsub_e σ) cargs
-  | Stmt.Method e m τs oe
-    => Stmt.Method e m (map (tsub_t σ) τs) $ option_map (tsub_e σ) oe
-  end.
+  Definition tsub_transition (transition : Parser.e) :=
+    match transition with
+    | Parser.Direct s => Parser.Direct s
+    | Parser.Select discriminee default cases =>
+        Parser.Select (tsub_e discriminee) default cases
+    end.
 
-Fixpoint tsub_s (σ : nat -> Expr.t) (s : Stmt.s) : Stmt.s :=
-  match s with
-  | Stmt.Skip
-  | Stmt.Exit => s
-  | Stmt.Invoke t es => Stmt.Invoke t $ map (tsub_e σ) es
-  | Stmt.Return e => Stmt.Return $ option_map (tsub_e σ) e
-  | Stmt.Transition e => Stmt.Transition $ tsub_transition σ e
-  | (lhs `:= rhs)%stmt
-    => (tsub_e σ lhs `:= tsub_e σ rhs)%stmt
-  | Stmt.Call fk args
-    => Stmt.Call (tsub_fun_kind σ fk) $ map (tsub_arg σ) args
-  | Stmt.Apply ci ext_args args =>
-      Stmt.Apply ci ext_args $ map (tsub_arg σ) args
-  | Stmt.Var e s
-    => Stmt.Var
-        (map_sum (tsub_t σ) (tsub_e σ) e)
-        $ tsub_s σ s
-  | (s₁ `; s₂)%stmt => (tsub_s σ s₁ `; tsub_s σ s₂)%stmt
-  | (If g Then tru Else fls)%stmt
-    => (If tsub_e σ g Then tsub_s σ tru Else tsub_s σ fls)%stmt
-  end.
+  Definition tsub_fun_kind (fk : Stmt.fun_kind) : Stmt.fun_kind :=
+    match fk with
+    | Stmt.Funct f τs oe
+      => Stmt.Funct f (map tsub_t τs) $ option_map tsub_e oe
+    | Stmt.Action a cargs
+      => Stmt.Action a $ map tsub_e cargs
+    | Stmt.Method e m τs oe
+      => Stmt.Method e m (map tsub_t τs) $ option_map tsub_e oe
+    end.
 
-Definition tsub_carg
-           (σ : nat -> Expr.t) (carg : TopDecl.constructor_arg)
-  : TopDecl.constructor_arg :=
-  match carg with
-  | TopDecl.CAName _ => carg
-  | TopDecl.CAExpr e => tsub_e σ e
-  end.
+  Fixpoint tsub_s (s : Stmt.s) : Stmt.s :=
+    match s with
+    | Stmt.Skip
+    | Stmt.Exit => s
+    | Stmt.Invoke t es => Stmt.Invoke t $ map tsub_e es
+    | Stmt.Return e => Stmt.Return $ option_map tsub_e e
+    | Stmt.Transition e => Stmt.Transition $ tsub_transition e
+    | (lhs `:= rhs)%stmt
+      => (tsub_e lhs `:= tsub_e rhs)%stmt
+    | Stmt.Call fk args
+      => Stmt.Call (tsub_fun_kind fk) $ map tsub_arg args
+    | Stmt.Apply ci ext_args args =>
+        Stmt.Apply ci ext_args $ map tsub_arg args
+    | Stmt.Var e s
+      => Stmt.Var
+          (map_sum tsub_t tsub_e e)
+          $ tsub_s s
+    | (s₁ `; s₂)%stmt => (tsub_s s₁ `; tsub_s s₂)%stmt
+    | (If g Then tru Else fls)%stmt
+      => (If tsub_e g Then tsub_s tru Else tsub_s fls)%stmt
+    end.
 
-Definition tsub_cparam
-         (σ : nat -> Expr.t) (ctor_type : TopDecl.it) : TopDecl.it :=
-  match ctor_type with
-  | TopDecl.ControlInstType extern_params params =>
-      TopDecl.ControlInstType
-        extern_params (map (tsub_param σ) params)
-  | TopDecl.ParserInstType extern_params params =>
-      TopDecl.ParserInstType
-        extern_params (map (tsub_param σ) params)
-  | TopDecl.PackageInstType => TopDecl.PackageInstType
-  | TopDecl.ExternInstType e => TopDecl.ExternInstType e
-  | TopDecl.EType t => tsub_t σ t
-  end.
+  Definition tsub_cparam
+             (ctor_type : TopDecl.it) : TopDecl.it :=
+    match ctor_type with
+    | TopDecl.ControlInstType extern_params params =>
+        TopDecl.ControlInstType
+          extern_params (map tsub_param params)
+    | TopDecl.ParserInstType extern_params params =>
+        TopDecl.ParserInstType
+          extern_params (map tsub_param params)
+    | TopDecl.PackageInstType => TopDecl.PackageInstType
+    | TopDecl.ExternInstType e => TopDecl.ExternInstType e
+    end.
 
-Definition tsub_arrowT
-           (σ : nat -> Expr.t)
-           '({| paramargs:=params; rtrns:=ret |} : Expr.arrowT) : Expr.arrowT :=
-  {| paramargs := map (tsub_param σ) params
-  ; rtrns := option_map (tsub_t σ) ret |}.
+  Definition tsub_arrowT
+             '({| paramargs:=params; rtrns:=ret |} : Expr.arrowT) : Expr.arrowT :=
+    {| paramargs := map tsub_param params
+    ; rtrns := option_map tsub_t ret |}.
+End Sub.
 
 Definition tsub_method
            (σ : nat -> Expr.t)
@@ -146,28 +148,35 @@ Definition tsub_Cd (σ : nat -> Expr.t) (d : Control.d) :=
 
 Definition tsub_d (σ : nat -> Expr.t) (d : TopDecl.d) : TopDecl.d :=
   match d with
-  | TopDecl.Instantiate cname type_args cargs =>
+  | TopDecl.Instantiate cname iname type_args cargs expr_cargs =>
       (* TODO theres something broken here, need to get type params for cname *)
       let type_args' := map (tsub_t σ) type_args in
-      let cargs' := map (tsub_carg σ) cargs in
-      TopDecl.Instantiate cname type_args' cargs'
-  | TopDecl.Extern ename tparams cparams methods =>
+      let expr_cargs' := map (tsub_e σ) expr_cargs in
+      TopDecl.Instantiate cname iname type_args' cargs expr_cargs'
+  | TopDecl.Extern ename tparams cparams expr_cparams methods =>
       let σ' := exts `^ tparams σ in
-      let cparams' := map (tsub_cparam σ') cparams in
+      let cparams' :=
+        List.map (FunUtil.map_snd $ tsub_cparam σ') cparams in
+      let expr_cparams' :=
+        map (tsub_t σ') expr_cparams in
       let methods' := Field.map (tsub_method σ') methods in
-      TopDecl.Extern ename tparams cparams' methods'
-  | TopDecl.Control cname cparams eparams params body apply_blk =>
-      let cparams' := map (tsub_cparam σ) cparams in
+      TopDecl.Extern ename tparams cparams' expr_cparams' methods'
+  | TopDecl.Control cname cparams expr_cparams eparams params body apply_blk =>
+      let cparams' := map (FunUtil.map_snd $ tsub_cparam σ) cparams in
+      let expr_cparams' :=
+        map (tsub_t σ) expr_cparams in
       let params' := map (tsub_param σ) params in
       let body' := map (tsub_Cd σ) body in
       let apply_blk' := tsub_s σ apply_blk in
-      TopDecl.Control cname cparams' eparams params' body' apply_blk'
-  | TopDecl.Parser pn cps eps ps strt sts =>
-      let cparams' := map (tsub_cparam σ) cps in
-      let params' := map (tsub_param σ) ps in
+      TopDecl.Control cname cparams' expr_cparams' eparams params' body' apply_blk'
+  | TopDecl.Parser pn cps expr_cparams eps ps strt sts =>
+      let cps' := map (FunUtil.map_snd $ tsub_cparam σ) cps in
+      let expr_cparams' :=
+        map (tsub_t σ) expr_cparams in
+      let ps' := map (tsub_param σ) ps in
       let start' := tsub_s σ strt in
       let states' := map (tsub_s σ) sts in
-      TopDecl.Parser pn cparams' eps params' start' states'
+      TopDecl.Parser pn cps' expr_cparams' eps ps' start' states'
   | TopDecl.Funct f tparams params body =>
       let σ' := exts `^ tparams σ in
       let cparams' := tsub_arrowT σ' params in
