deps/poulet4/lib/P4cub/Syntax/Syntax.v
@@ -2,7 +2,7 @@ From Poulet4 Require Export P4cub.Syntax.AST
      P4cub.Syntax.CubNotations
      P4cub.Syntax.IndPrincip
      P4cub.Syntax.Equality
-     P4cub.Syntax.Auxilary
+     P4cub.Syntax.Auxiliary
      P4cub.Syntax.InferMemberTypes
      P4cub.Syntax.P4Field
      P4cub.Syntax.Substitution.
